Partial passes

src/Partial.fst
@@ -3,51 +3,53 @@ module Partial
 open FStar.Set
 open SetExtra
 
-type t (key:Type) (value:Type) = list (key * value)
+type t (key:eqtype) (value:eqtype) = list (key * value)
 
-val keys     : #key:Type -> #value:Type -> t key value -> Tot (set key)
-val vals     : #key:Type -> #value:Type -> t key value -> Tot (set value)
-val defined  : #key:Type -> #value:Type -> t key value -> key -> Tot bool
-val find     : #key:Type -> #value:Type -> t key value -> key -> Tot (option value)
-val find_def : #key:Type -> #value:Type -> t key value -> key -> value -> Tot value
-val update   : #key:Type -> #value:Type -> t key value -> key -> value -> Tot (t key value)
-val remove   : #key:Type -> #value:Type -> t key value -> key -> Tot (t key value)
-val totalize : #key:Type -> #value:Type -> t key value -> value -> Tot (Total.t key value)
-val mapVals  : #key:Type -> #value:Type -> #value':Type -> 
+val keys     : #key:eqtype -> #value:eqtype -> t key value -> Tot (set key)
+val vals     : #key:eqtype -> #value:eqtype -> t key value -> Tot (set value)
+val defined  : #key:eqtype -> #value:eqtype -> t key value -> key -> Tot bool
+val find     : #key:eqtype -> #value:eqtype -> t key value -> key -> Tot (option value)
+val find_def : #key:eqtype -> #value:eqtype -> t key value -> key -> value -> Tot value
+val update   : #key:eqtype -> #value:eqtype -> t key value -> key -> value -> Tot (t key value)
+val remove   : #key:eqtype -> #value:eqtype -> t key value -> key -> Tot (t key value)
+val totalize : #key:eqtype -> #value:eqtype -> t key value -> value -> Tot (Total.t key value)
+val mapVals  : #key:eqtype -> #value:eqtype -> #value':eqtype -> 
 	       (value -> Tot value') -> t key value -> Tot (t key value')
 
-let rec keys m = match m with
-  | []    -> fun _ -> false
-  | x::xs -> fun y -> (fst x) = y || keys xs y
+let rec keys #k #v m = match m with
+  | []   -> empty
+  | x::xs -> ins (fst x) (keys xs)
 
-let rec vals m = match m with
-  | []    -> fun _ -> false
-  | x::xs -> fun y -> (snd x) = y || vals xs y
+let rec vals #k #v m = match m with
+  | []   -> empty
+  | x::xs -> ins (snd x) (vals xs)
 
-let defined m k = mem k (keys m)
+let defined #k #v m key = mem key (keys m)
 
-let rec find m k = List.assocT k m
+let rec find #k #v m key = match m with //FStar.List.Tot.assoc key m
+  | []   -> None
+  | x::xs -> if (fst x) = key then Some (snd x) else find xs key
 
-let rec find_def m k dval = match find m k with
+let rec find_def #k #v m key dval = match find m key with
   | None -> dval 
   | Some v -> v
 
-let rec update m k v = match m with
-    | [] -> [(k, v)]
-    | (k', v')::xs -> if k = k' then (k, v)::xs else (k', v')::(update xs k v)
+let rec update #k #v m key vl = match m with
+    | [] -> [(key, vl)]
+    | (key', vl')::xs -> if key = key' then (key, vl)::xs else (key', vl')::(update xs key vl)
 
-let rec remove m k = match m with
+let rec remove #k #v m key = match m with
   | [] -> []
-  | (k', v')::xs -> if k = k' then xs else (k', v')::(remove xs k)
+  | (key', v')::xs -> if key = key' then xs else (key', v')::(remove xs key)
 
-let totalize m dval =
+let totalize #k #v m dval =
   { Total.elts = m;
     Total.dval = dval }
 
-let mapVals f m = List.mapT (fun (k, v) -> (k, f v)) m
+let mapVals #k #v #u f m = FStar.List.mapT (fun (key, v) -> (key, f v)) m
 
 (** Verification utilities *)
-val lookup   : #key:Type -> #value:Type -> m:t key value -> k:key{defined m k} -> Tot value
+val lookup   : #key:eqtype -> #value:eqtype -> m:t key value -> k:key{defined m k} -> Tot value
 
-let rec lookup m k = match m with
-  | (k', v)::xs -> if k = k' then v else lookup xs k
+let rec lookup #k #v m key = match m with
+  | (key', v)::xs -> if key = key' then v else lookup xs key
